substitute.v
@@ -1,0 +1,426 @@
+(* -*- mode: coq -*- *)
+(* Time-stamp: <2014/8/23 21:0:44> *)
+(*
+  substitute.v 
+  - mathink : Author
+ *)
+
+(* Program libraries for [Program] *)
+(* Map Skelton *)
+Require Import
+Ssreflect.ssreflect
+Ssreflect.ssrfun
+Ssreflect.ssrbool
+Ssreflect.eqtype.
+
+Set Implicit Arguments.
+Unset Strict Implicit.
+
+Require Import MSL.lambda.
+
+Delimit Scope map with map_scope.
+Open Scope map_scope.
+Unset Strict Implicit.
+Import Prenex Implicits.
+
+(* Notations for Maybe *)
+Definition bind {X Y: Type}(f: X -> option Y)(m: option X): option Y :=
+  if m is Some x then f x else None.
+Notation emb := Some.
+Notation "m >>= f" := (bind f m) (at level 65, left associativity).
+Notation "m >> p" := (bind (fun _ => p) m) (at level 65, left associativity).
+Notation "x <- m ; p" := (m >>= fun x => p) (at level 60, right associativity).
+Notation "(: x , y :) <- m ; p" := (m >>= fun tup:_*_ => let: (x,y) := tup in p) (at level 60, right associativity).
+Notation "'do' m" := m (at level 100, right associativity).
+Notation "'mlet' x := m ; p" := (x <- emb m ; p) (at level 60, right associativity).
+
+Section HoleFilling.
+  Open Scope map_scope.
+  Context {T: eqType}.
+
+  Notation "[=]" := (box T).
+  Let sexp := sexp T.
+  Let lambda := lambda T.
+
+  Arguments asL {T}(s H): rename.
+
+  Check (fun s (b: is_true (wfb 0 s)) =>(elimT (wfbP 0 s) b)).
+  Notation "[ 'L' s | b ]" :=
+    (Lam (introT (isLbP s) (elimT (isLbP s) b)))
+  (at level 0, format "[ 'L' s | b ]"): map_scope.
+  Notation "'L.' s" := (asL s _)
+  (at level 0, format "'L.' s"): map_scope.
+  Notation "[ 'S' M ]" := (body M)
+  (at level 0, format "[ 'S' M ]"): map_scope.
+  Notation "'S.' M" := (body M)
+  (at level 0, format "'S.' M"): map_scope.
+  Definition asL (s: sexp): 0#s -> lambda :=
+    fun H => Lam (introT (isLbP s) (wf_sexp_is_lambda H)).
+
+  Fixpoint HF_aux (P: lambda)(m: map)(s: sexp){struct s}: option sexp :=
+    match m, s with
+      | 1, box => Some S.P
+      | 0, box => Some [=]
+      | 0, free x => Some (free x)
+      | 1, free x => None
+      | 0, M@N =>
+       match HF_aux P 0 M, HF_aux P 0 N with
+         | Some MmP, Some NnP  => Some (MmP@NnP)
+         | _, _  => None end
+      | minl m, M@N =>
+       match HF_aux P m M, HF_aux P 0 N with
+         | Some MmP, Some NnP  => Some (MmP@NnP)
+         | _, _  => None end
+      | minr n, M@N =>
+       match HF_aux P 0 M, HF_aux P n N with
+         | Some MmP, Some NnP  => Some (MmP@NnP)
+         | _, _  => None end
+      | mcons m n, M@N =>
+       match HF_aux P m M, HF_aux P n N with
+         | Some MmP, Some NnP  => Some (MmP@NnP)
+         | _, _  => None end
+      | m, n\N =>
+        if wfb n N && orthb n m then
+          if HF_aux P m N is Some NmP then Some (n\NmP) else None
+        else None
+      |  _,_  => None
+    end.
+
+  Functional Scheme HF_aux_ind := Induction for HF_aux Sort Prop.
+
+  Lemma HF_0 M (P: lambda): 0#M -> emb M = HF_aux P 0 M.
+  Proof.
+    elim: M => [x||M1 IH1 M2 IH2|m M IH] Hwf //=.
+    - rewrite -mapp_00_0 in Hwf; inversion Hwf; subst.
+      rewrite H; rewrite -mapp_00_0 in H.
+      by move: H H2 H3 => /eqP; rewrite mapp_injective;
+        move=> /andP [/eqP -> /eqP ->] H1 H2;
+          rewrite -(IH1 H1) -(IH2 H2). 2!emb_bind //=.
+    - rewrite orthb_symm //= andbT.
+      inversion Hwf; subst.
+      by move: H3 => /wfbP ->; rewrite -(IH H1).
+  Qed.
+      
+(*   Lemma orth_wf_HF_wf m1 m2 t t1 P: *)
+(*     m1!m2 -> m1#t -> emb t1 = HF_aux P m1 t -> m2#t1. *)
+(*   Proof. *)
+(*     move: m2 t1. *)
+(*     pattern (HF_aux P m1 t); apply HF_aux_ind => // m0 s0. *)
+(*     - move=> _{m0} x _{s0} m s Hor Hwf [] -> //=. *)
+(*       inversion Hor. *)
+(*     elim/HF_aux_ind: P t /(HF_aux P m1 t). *)
+(* Check HF_aux_ind. *)
+(*     elim=> [m|n|m n m' n' Ho IH Ho' IH'] Hwf Heq /=. *)
+(*     - elim: t m Hwf Heq => [x||s1 IHs1 s2 IHs2|m s1 IH] /=. *)
+(*       + move=> m Hwfm; inversion Hwfm; subst. *)
+(*         by move=> Heq; apply emb_mono in Heq; subst. *)
+(*       + move=> m Hwfm; inversion Hwfm; subst. *)
+(*         * by move=> Heq; apply emb_mono in Heq; subst. *)
+(*         * move=> Heq; apply emb_mono in Heq; subst. *)
+(*           apply lambda_is_wf. *)
+(*       + move=> m Hwfm; inversion Hwfm; subst. *)
+(*         destruct m0, n; simpl in *. *)
+(*         * rewrite -(HF_0 _ H2) -(HF_0 _ H3) 2!emb_bind; *)
+(*           by move=> Heq; apply emb_mono in Heq; move: Heq => ->. *)
+(*         * rewrite -(HF_0 _ H2) emb_bind. *)
+
+  Lemma HF_aux_wf s m P:
+    m#s -> exists t: sexp, emb t = HF_aux P m s/\isLb t.
+  Proof.
+    elim=> [y|||m1 m2 s1 s2 H1 IH1 H2 IH2|m1 m2 t H1 IH1 H2 IH2 Horth] .
+    - exists (free y); repeat split; constructor.
+    - by exists [=]; repeat split; constructor.
+    - by exists (S.P); repeat split; try constructor; destruct P.
+    - move: IH1 IH2 => [t1 [Heq1 HL1]] [t2 [Heq2 HL2]].
+      exists (t1@t2).
+      destruct m1, m2; simpl in *;
+      (rewrite -Heq1 -Heq2;
+       repeat split; try done; last by apply /andP; split).
+    - move: IH1 IH2 => [t1 [Heq1 HL1]] [t2 [Heq2 HL2]].
+      exists (m2\t1); split.
+      + simpl HF_aux.
+        rewrite -Heq1 /=.
+        case: (m2!P m1) => [Hor|Hnor]; rewrite ?andbT ?andbF.
+        * case: (m2#P t) => [Hwf|Hnwf]; rewrite ?andbT.
+          clear Heq1 H1 Horth Hor.
+          destruct m1; try done.
+          destruct m0; try done.
+        * destruct m1; try done.
+      + apply orth_symm in Horth; contradiction.
+    - apply/isLbP; apply labs; first by apply/isLbP.
+  (* have: m1!m2 -> m1#t -> emb t1 = HF_aux t m1 P -> m2#t1 *)
+      Abort.
+  Qed.
+
+  Notation "[ M '_' m { P } ]" := (HF_ M m P).
+
+
+  Program Fixpoint HoleFill (s: sexp)(m: map)(s: lambda): F lambda :=
+    match M , m return F lambda with
+      | Lam (free x) _, 0 => emb L.(free x)
+      | Lam box _, 1 => emb P
+      | Lam box _, 0 => emb L.[]
+      | Lam (M@N) H, 0 =>
+        do mlet m := 0;
+           mlet n := 0;
+           MmP <- HoleFill L.M m P;
+           NnP <- HoleFill L.N n P;
+           emb L.(S.MmP @ S.NnP)
+      | _, _ => failure lambda
+    end; try by constructor.
+    Proof.
+      - rewrite -mapp_00_0; apply wf_mapp_app; apply lambda_is_wf.
+      - move: H => /isLbP.
+        destruct term.
+apply lambda_is_wf.
+
+      | M@N, minl m =>
+        do mlet n := 0;
+           MmP <- HoleFill L.M m P;
+           NnP <- HoleFill L.N n P;
+           emb L.(S.MmP @ S.NnP)
+      | M@N, minr n =>
+        do mlet m := 0;
+           MmP <- HoleFill M m P;
+           NnP <- HoleFill N n P;
+           emb (MmP@NnP)
+       | M@N, mcons m n =>
+         do MmP <- HoleFill M m P;
+            NnP <- HoleFill N n P;
+            emb (MmP@NnP)
+       | n\N, m =>
+         do NmP <- HoleFill N m P;
+            emb (n\NmP)
+      | _, _ => failure lambda
+    end).
+          | _,_ => failure sexP
+        end.
+
+      Notation "[ M '_' m { P } ]" := (HoleFill M m P).
+
+      (*      Lemma wf_wf m x: 0#x -> m#x.
+      Proof.
+        move=> H0x; move: x H0x m.
+        elim=> [y||s IHs t IHt|m s IHs] Hwf m'; try constructor. *)
+
+      (* Lemma HoleFill_wf m M N: *)
+      (*   (exists x, emb x = HoleFill M m N) -> m#M. *)
+
+      Lemma HoleFill_wf m M N:
+        m#M -> 0#N -> exists x, 0#x /\ emb x = HoleFill M m N.
+      Proof.
+        move=> HmM H0N.
+        elim: HmM =>  //= [x||
+                          | m1 m2 s t H1 IH1 H2 IH2
+                          | m1 m2 s H1 IH1 H2 IH2] /=.
+        - exists (free x); split; try by constructor.
+        - exists box; split; try by constructor.
+        - exists N; split; done.
+          move: IH1 IH2 => [x1 [Hx1 Heq1]] [x2 [Hx2 Heq2]] /=.
+          exists (x1@x2); split;
+          first (rewrite -mapp_00_0; apply wf_mapp_app; done).
+          case: m1 H1 Heq1 => /=.
+          + case: m2 H2 Heq2 => /=.
+            * move=> _ Heq1 _ Heq2.
+                by rewrite emb_bind emb_bind
+                   -Heq1 -Heq2 emb_bind emb_bind.
+            * move=> m' _ Heq1 _ Heq2.
+                by rewrite emb_bind -Heq1 -Heq2 emb_bind emb_bind.
+          + case: m2 H2 Heq2 => /=.
+            * move=> _ Heq1 n' _ Heq2.
+                by rewrite emb_bind -Heq1 -Heq2 emb_bind emb_bind.
+            * move=> m' _ Heq1 n' _ Heq2.
+                by rewrite -Heq1 -Heq2 emb_bind emb_bind.
+        - move: IH1 IH2 => [x1 [Hx1 Heq1]] [x2 [Hx2 Heq2]] Horth.
+          rewrite -Heq1 emb_bind.
+          exists (m2\x1); split; last done.
+          apply wf_abs; first done; try by constructor.
+          (*   Heq2 : emb x2 = [s _ m2 {N}] means m2#x1 *)
+
+      Fixpoint mapf (x: T)(s: sexp): map :=
+        match s with
+          | free y => if x == y then 1 else 0
+          | box => 0
+          | M@N => mapf x M*mapf x N
+          | m\M => mapf x M
+        end.
+
+      Fixpoint skelf (x: T)(s: sexp): sexp :=
+        match s with
+          | free y => if x == y then box else free y
+          | box => box
+          | M@N => skelf x M@skelf x N
+          | m\M => m\skelf x M
+        end.
+
+      Definition lam (x: T)(M: sexp) := mapf x M\skelf x M.
+
+      Lemma mapp_0 m n: m*n = 0 -> m = 0 /\ n = 0.
+      Proof.
+        case: m => [|m] /=; case: n => [| n] /=; try done.
+      Qed.
+
+      Lemma wf_skelf m x s: m#s -> m#skelf x s.
+      Proof.
+        elim=> [y|||m1 m2 s1 s2 H1 IH1 H2 IH2|m1 m2 t H1 IH1 H2 IH2 H] /=;
+          try by constructor.
+        - case: (x == y) => /=; try by constructor.
+      Qed.
+
+
+(*      Lemma orth_mapf m x s: 0#s -> 0!m -> (mapf x s)!m.
+        elim: s => [y||s IHs t IHt|n s IHs] /= Hwf Horth;
+                  try by constructor.
+        - case: (x == y) => /=; try by constructor.
+          simpl.
+        move=> Horth; move: Horth x s.
+        elim=> [m'|n'|m1 n1 m2 n2 H1 IH1 H2 IH2] x s; try by constructor.
+      Lemma orth_mapf m x s: 0!m -> mapf x s!m.
+      Proof.
+        move=> Horth; move: Horth x s.
+        elim=> [_|n|m1 n1 m2 n2 H1 IH1 H2 IH2]; try by constructor.
+        - case: (x == y) => /=; try by constructor.
+      Qed.
+       *)
+
+      (*
+      Lemma map_skeleton_aux:
+        forall x m M,
+          m#M ->
+          m*mapf x M # skelf x M -> mapf x M # m\skelf x M.
+      Proof.
+        move=> x m M Hwf.
+        elim: Hwf => [y||
+                     |m1 m2 s1 s2 H1 IH1 H2 IH2
+                     |m1 m2 s H1 IH1 H2 IH2 Horth] /=;
+          try by constructor.
+        - case: (x == y) => /=; try by constructor.
+          + move=> H; inversion H.
+          + move=> H; inversion H.
+            apply wf_abs; try by constructor.
+        - move=> H; apply wf_abs; try by constructor.
+        - move=> H; apply wf_abs; try by constructor.
+        - move=> H; inversion H; subst.
+          move: H3 => /eqP; rewrite mapp_injective;
+            move=> -/andP [-/eqP Heq1 -/eqP Heq2]; subst.
+          apply wf_abs; try done.
+          apply wf_mapp_app; try done.
+          + apply wf_mapp_app; try done.
+
+
+        move=> x m M; simpl; auto.
+      Qed.
+       *)
+
+      Definition substitute (M: sexp)(x: T)(p: sexp) :=
+        HoleFill (skelf x M) (mapf x M) p.
+
+      Lemma substitute_app M N x P:
+        substitute (M@N) x P = do MxP <- substitute M x P;
+                                  NxP <- substitute N x P;
+                                  emb (MxP@NxP).
+      Proof.
+        rewrite /substitute //=.
+        case: (mapf x M) => //=.
+        - case: (mapf x N) => //=.
+          + by rewrite emb_bind emb_bind.
+          + by move=> m; rewrite emb_bind.
+        - move=> m.
+          case: (mapf x N) => //=.
+          + by rewrite emb_bind.
+      Qed.
+
+      Lemma substitute_abs m M x P:
+        substitute (m\M) x P = do MxP <- substitute M x P;
+                                  emb (m\MxP).
+      Proof.
+        rewrite /substitute //=.
+      Qed.
+
+
+      Lemma fresh_on_skelf x P:
+        fresh_on x P -> skelf x P = P.
+      Proof.
+        elim: P => //= [y|s IHs t IHt| m s IHs] /=.
+        - apply ifN_eq.
+        - by move=> /andP [Hs Ht]; rewrite (IHs Hs) (IHt Ht).
+        - by move=> H; rewrite (IHs H).
+      Qed.
+
+      Lemma fresh_on_mapf x P:
+        fresh_on x P -> mapf x P = 0.
+      Proof.
+        elim: P => //= [y|s IHs t IHt] /=.
+        - apply ifN_eq.
+        - by move=> /andP [Hs Ht]; rewrite (IHs Hs) (IHt Ht).
+      Qed.
+
+      Lemma HF_0 P M: emb P = HoleFill P 0 M.
+      Proof.
+        { elim: P => [x||s IHs t IHt|m s IHs] //=.
+          - rewrite emb_bind emb_bind //= -IHs -IHt.
+            rewrite emb_bind emb_bind //=.
+          - by rewrite -IHs emb_bind. }
+      Qed.
+
+      Lemma substitute_lemma x y P M N:
+        x <> y -> fresh_on x P ->
+        (do MxN <- substitute M x N;
+            substitute MxN y P)
+        =
+        (do MyP <- substitute M y P;
+            NyP <- substitute N y P;
+            substitute MyP x NyP).
+      Proof.
+        move=> Hneq Hfresh.
+        rewrite /substitute; induction M; move=> //=.
+        - case Hxx0: (x == x0) => //=.
+          + rewrite emb_bind //=.
+            case Hyy0: (y == x0) => //=.
+            * move: Hxx0 Hyy0 => /eqP Hxx0 /eqP Hyy0 //=; subst.
+                by elim Hneq.
+            * by rewrite emb_bind //= Hxx0 //= bind_emb.
+          + rewrite emb_bind //=.
+            case Hyy0: (y == x0) => //=.
+            * rewrite emb_bind //=.
+              rewrite (fresh_on_mapf Hfresh)
+                      (fresh_on_skelf Hfresh) //=.
+              { elim: N => [x1||s IHs t IHt| m s IHs] //=.
+                - case Hyx1: (y == x1) => //=.
+                  + rewrite emb_bind.
+                    apply: (HF_0 P P).
+                  + rewrite emb_bind.
+                    apply: (HF_0 P _).
+                - rewrite emb_bind.
+                  apply: (HF_0 P _).
+                - destruct (mapf y s); simpl.
+                  + destruct (mapf y t); simpl.
+                    * rewrite emb_bind emb_bind.
+                      by rewrite -(HF_0 _ P) -(HF_0 _ P)
+                        emb_bind emb_bind emb_bind -(HF_0 _ _).
+                    * rewrite emb_bind -(HF_0 _ _) emb_bind //=.
+                      rewrite bind_assoc IHt.
+                      apply bind_subst; try done.
+                      by move=> x1;
+                          rewrite emb_bind -(HF_0 _ _) -(HF_0 _ _).
+                  + destruct (mapf y t); simpl.
+                    * rewrite emb_bind bind_assoc IHs.
+                      apply bind_subst; try done.
+                      move=> x1.
+                      rewrite bind_assoc -(HF_0 _ _) IHt.
+                      apply bind_subst; try done.
+                      move=> x2.
+                      by rewrite emb_bind -(HF_0 _ _) -(HF_0 _ _).
+                    * rewrite bind_assoc IHs.
+                      apply bind_subst; try done.
+                      move=> x1.
+                      rewrite bind_assoc -(HF_0 _ _) IHt.
+                      apply bind_subst; try done.
+                      move=> x2.
+                      by rewrite emb_bind -(HF_0 _ _) -(HF_0 _ _).
+                - rewrite bind_assoc IHs.
+                  apply bind_subst; try done.
+                  move=> x1.
+                    by rewrite emb_bind -(HF_0 _ _) -(HF_0 _ _). }
+            * rewrite emb_bind //= Hxx0 /=.
+              
